Everything in the internal folder is now in the MyLean.DHashMap.Internal namespace

Hashmap/DHashMap/AdditionalOperations.lean
@@ -10,6 +10,8 @@ This file defines operations on `DHashMap` which cannot be defined in `Basic.lea
 This file will have more imports than `Basic.lean` once everything is properly untangled.
 -/
 
+open MyLean.DHashMap.Internal
+
 set_option autoImplicit false
 
 universe u v w
@@ -20,20 +22,22 @@ namespace MyLean.DHashMap
 
 namespace Raw
 
+open Internal.Raw
+
 theorem WF.filterMap [BEq α] [Hashable α] {m : Raw α β} (h : m.WF) {f : (a : α) → β a → Option (δ a)} :
     (m.filterMap f).WF := by
-  simpa only [filterMap_eq h] using .wf (Raw₀.filterMap f ⟨m, h.size_buckets_pos⟩).2 (.filterMap h.out)
+  simpa only [filterMap_eq h] using .wf (Raw₀.filterMap f ⟨m, h.size_buckets_pos⟩).2 (Internal.Raw.WFImp.filterMap h.out)
 
 theorem WF.map [BEq α] [Hashable α] {m : Raw α β} (h : m.WF) {f : (a : α) → β a → δ a} :
     (m.map f).WF := by
-  simpa only [map_eq h] using .wf (Raw₀.map f ⟨m, h.size_buckets_pos⟩).2 (.map h.out)
+  simpa only [map_eq h] using .wf (Raw₀.map f ⟨m, h.size_buckets_pos⟩).2 (Internal.Raw.WFImp.map h.out)
 
 end Raw
 
 @[inline] def filterMap [BEq α] [Hashable α] (f : (a : α) → β a → Option (δ a)) (m : DHashMap α β) : DHashMap α δ :=
-  ⟨Raw₀.filterMap f ⟨m.1, m.2.size_buckets_pos⟩, .wf (Raw₀.filterMap f ⟨m.1, m.2.size_buckets_pos⟩).2 m.2.out.filterMap⟩
+  ⟨Raw₀.filterMap f ⟨m.1, m.2.size_buckets_pos⟩, .wf (Raw₀.filterMap f ⟨m.1, m.2.size_buckets_pos⟩).2 (Internal.Raw.WFImp.filterMap m.2.out)⟩
 
 @[inline] def map [BEq α] [Hashable α] (f : (a : α) → β a → δ a) (m : DHashMap α β) : DHashMap α δ :=
-  ⟨Raw₀.map f ⟨m.1, m.2.size_buckets_pos⟩, .wf (Raw₀.map f ⟨m.1, m.2.size_buckets_pos⟩).2 m.2.out.map⟩
+  ⟨Raw₀.map f ⟨m.1, m.2.size_buckets_pos⟩, .wf (Raw₀.map f ⟨m.1, m.2.size_buckets_pos⟩).2 (Internal.Raw.WFImp.map m.2.out)⟩
 
 end MyLean.DHashMap
