Hashmap/DHashMap/Internal/AssocList/Lemmas.lean
@@ -15,7 +15,9 @@ universe w v u
 
 variable {α : Type u} {β : α → Type v} {γ : α → Type w} {δ : Type w} {m : Type w → Type w} [Monad m]
 
-namespace MyLean.AssocList
+namespace MyLean.DHashMap.Internal.AssocList
+
+open Internal.List
 
 @[simp] theorem toList_nil : (nil : AssocList α β).toList = [] := rfl
 @[simp] theorem toList_cons {l : AssocList α β} {a : α} {b : β a} : (l.cons a b).toList = ⟨a, b⟩ :: l.toList := rfl
@@ -24,7 +26,6 @@ namespace MyLean.AssocList
 theorem foldl_eq {f : δ → (a : α) → β a → δ} {init : δ} {l : AssocList α β} :
     l.foldl f init = l.toList.foldl (fun d p => f d p.1 p.2) init := by
   induction l generalizing init <;> simp_all [foldl, Id.run, foldlM]
-
 
 @[simp]
 theorem length_eq {l : AssocList α β} : l.length = l.toList.length := by
@@ -37,34 +38,34 @@ theorem length_eq {l : AssocList α β} : l.length = l.toList.length := by
     simp [ih, Nat.add_assoc, Nat.add_comm n 1]
 
 @[simp]
-theorem get?_eq {β : Type v} [BEq α] {l : AssocList α (fun _ => β)} {a : α} : l.get? a = l.toList.getValue? a := by
+theorem get?_eq {β : Type v} [BEq α] {l : AssocList α (fun _ => β)} {a : α} : l.get? a = getValue? a l.toList := by
   induction l <;> simp_all [get?, List.getValue?]
 
 @[simp]
-theorem getCast?_eq [BEq α] [LawfulBEq α] {l : AssocList α β} {a : α} : l.getCast? a = l.toList.getValueCast? a := by
+theorem getCast?_eq [BEq α] [LawfulBEq α] {l : AssocList α β} {a : α} : l.getCast? a = getValueCast? a l.toList := by
   induction l <;> simp_all [getCast?, List.getValueCast?]
 
 @[simp]
-theorem contains_eq [BEq α] {l : AssocList α β} {a : α} : l.contains a = l.toList.containsKey a := by
+theorem contains_eq [BEq α] {l : AssocList α β} {a : α} : l.contains a = containsKey a l.toList := by
   induction l <;> simp_all [contains, List.containsKey]
 
 @[simp]
 theorem getCast_eq [BEq α] [LawfulBEq α] {l : AssocList α β} {a : α} {h} :
-    l.getCast a h = l.toList.getValueCast a (contains_eq.symm.trans h) := by
+    l.getCast a h = getValueCast a l.toList (contains_eq.symm.trans h) := by
   induction l
   · simp [contains] at h
   · next k v t ih => simp only [getCast, toList_cons, List.getValueCast_cons, ih]
 
 @[simp]
 theorem get_eq {β : Type v} [BEq α] {l : AssocList α (fun _ => β)} {a : α} {h} :
-    l.get a h = l.toList.getValue a (contains_eq.symm.trans h) := by
+    l.get a h = getValue a l.toList (contains_eq.symm.trans h) := by
   induction l
   · simp [contains] at h
   · next k v t ih => simp only [get, toList_cons, List.getValue_cons, ih]
 
 @[simp]
 theorem getCastD_eq [BEq α] [LawfulBEq α] {l : AssocList α β} {a : α} {fallback : β a} :
-    l.getCastD a fallback = l.toList.getValueCastD a fallback := by
+    l.getCastD a fallback = getValueCastD a l.toList fallback := by
   induction l
   · simp [getCastD, List.getValueCastD]
   · simp_all [getCastD, List.getValueCastD, List.getValueCastD, List.getValueCast?_cons,
@@ -72,7 +73,7 @@ theorem getCastD_eq [BEq α] [LawfulBEq α] {l : AssocList α β} {a : α} {fall
 
 @[simp]
 theorem getD_eq {β : Type v} [BEq α] {l : AssocList α (fun _ => β)} {a : α} {fallback : β} :
-    l.getD a fallback = l.toList.getValueD a fallback := by
+    l.getD a fallback = getValueD a l.toList fallback := by
   induction l
   · simp [getD, List.getValueD]
   · simp_all [getD, List.getValueD, List.getValueD, List.getValue?_cons, apply_bif (fun x => Option.getD x fallback)]
@@ -83,7 +84,7 @@ theorem panicWithPosWithDecl_eq [Inhabited α] {modName declName line col msg} :
 
 @[simp]
 theorem getCast!_eq [BEq α] [LawfulBEq α] {l : AssocList α β} {a : α} [Inhabited (β a)] :
-    l.getCast! a = l.toList.getValueCast! a := by
+    l.getCast! a = getValueCast! a l.toList := by
   induction l
   · simp [getCast!, List.getValueCast!]
   · simp_all [getCast!, List.getValueCast!, List.getValueCast!, List.getValueCast?_cons,
@@ -91,25 +92,23 @@ theorem getCast!_eq [BEq α] [LawfulBEq α] {l : AssocList α β} {a : α} [Inha
 
 @[simp]
 theorem get!_eq {β : Type v} [BEq α] [Inhabited β] {l : AssocList α (fun _ => β)} {a : α} :
-    l.get! a = l.toList.getValue! a := by
+    l.get! a = getValue! a l.toList := by
   induction l
   · simp [get!, List.getValue!]
   · simp_all [get!, List.getValue!, List.getValue!, List.getValue?_cons, apply_bif Option.get!]
 
 @[simp]
 theorem toList_replace [BEq α] {l : AssocList α β} {a : α} {b : β a} :
-    (l.replace a b).toList = l.toList.replaceEntry a b := by
+    (l.replace a b).toList = replaceEntry a b l.toList := by
   induction l
   · simp [replace]
   · next k v t ih => cases h : k == a <;> simp_all [replace, List.replaceEntry_cons]
 
 @[simp]
-theorem toList_remove [BEq α] {l : AssocList α β} {a : α} : (l.remove a).toList = l.toList.removeKey a := by
+theorem toList_remove [BEq α] {l : AssocList α β} {a : α} : (l.remove a).toList = removeKey a l.toList := by
   induction l
   · simp [remove]
   · next k v t ih => cases h : k == a <;> simp_all [remove, List.removeKey_cons]
-
-open List
 
 theorem toList_filterMap {f : (a : α) → β a → Option (γ a)} {l : AssocList α β} :
     Perm (l.filterMap f).toList (l.toList.filterMap fun p => (f p.1 p.2).map (⟨p.1, ·⟩)) := by
@@ -120,12 +119,12 @@ theorem toList_filterMap {f : (a : α) → β a → Option (γ a)} {l : AssocLis
   induction l' generalizing l
   · simpa [filterMap.go] using Perm.refl _
   · next k v t ih =>
-    simp only [filterMap.go, toList_cons, filterMap_cons]
+    simp only [filterMap.go, toList_cons, List.filterMap_cons]
     split
     · next h => exact (ih _).trans (by simpa [h] using Perm.refl _)
     · next h =>
       refine (ih _).trans ?_
-      simp only [toList_cons, cons_append]
+      simp only [toList_cons, List.cons_append]
       exact perm_middle.symm.trans (by simpa [h] using Perm.refl _)
 
 theorem toList_map {f : (a : α) → β a → γ a} {l : AssocList α β} :
@@ -137,7 +136,7 @@ theorem toList_map {f : (a : α) → β a → γ a} {l : AssocList α β} :
   induction l' generalizing l
   · simpa [map.go] using Perm.refl _
   · next k v t ih =>
-    simp only [map.go, toList_cons, map_cons]
+    simp only [map.go, toList_cons, List.map_cons]
     refine (ih _).trans ?_
     simpa using perm_middle.symm
 
@@ -150,9 +149,9 @@ theorem toList_filter {f : (a : α) → β a → Bool} {l : AssocList α β} :
   induction l' generalizing l
   · simpa [filter.go] using Perm.refl _
   · next k v t ih =>
-    simp only [filter.go, toList_cons, filter_cons, cond_eq_if]
+    simp only [filter.go, toList_cons, List.filter_cons, cond_eq_if]
     split
     · exact (ih _).trans (by simpa using perm_middle.symm)
     · exact ih _
 
-end MyLean.AssocList
+end MyLean.DHashMap.Internal.AssocList
