Hashmap/DHashMap/Internal/Model.lean
@@ -9,7 +9,6 @@ import Hashmap.ForUpstream
 import Hashmap.Leftovers
 import Hashmap.DHashMap.Internal.AssocList.Lemmas
 
-open MyLean.DHashMap.Internal
 
 /-!
 In this file we define functions for manipulating a hash map based on operations defined in terms of their buckets.
@@ -24,7 +23,9 @@ universe u v w
 
 variable {α : Type u} {β : α → Type v} {γ : Type w} {δ : α → Type w}
 
-namespace MyLean.DHashMap
+namespace MyLean.DHashMap.Internal
+
+open Internal.List
 
 /-! # Setting up the infrastructure -/
 
@@ -67,14 +68,12 @@ theorem size_withComputedSize {self : Array (AssocList α β)} :
 theorem buckets_withComputedSize {self : Array (AssocList α β)} :
     (withComputedSize self).buckets = self := rfl
 
-open List
-
 theorem exists_bucket_of_uset [BEq α] [Hashable α]
   (self : Array (AssocList α β)) (i : USize) (hi : i.toNat < self.size) (d : AssocList α β) :
     ∃ l, Perm (toListModel self) (self[i.toNat].toList ++ l) ∧
       Perm (toListModel (self.uset i d hi)) (d.toList ++ l) ∧
       (∀ [LawfulHashable α], IsHashSelf self →
-        ∀ k : α, (mkIdx self.size (by omega) (hash k)).1.toNat = i.toNat → l.containsKey k = false) := by
+        ∀ k : α, (mkIdx self.size (by omega) (hash k)).1.toNat = i.toNat → containsKey k l = false) := by
   have h₀ : 0 < self.size := by omega
   obtain ⟨l₁, l₂, h₁, h₂, h₃⟩ := Array.exists_of_update self i d hi
   refine ⟨l₁.bind AssocList.toList ++ l₂.bind AssocList.toList, ?_, ?_, ?_⟩
@@ -85,7 +84,7 @@ theorem exists_bucket_of_uset [BEq α] [Hashable α]
   · intro _ h k
     rw [← Decidable.not_imp_not]
     intro hk
-    simp only [Bool.not_eq_false, containsKey_eq_true_iff_exists_mem, mem_append, mem_bind] at hk
+    simp only [Bool.not_eq_false, containsKey_eq_true_iff_exists_mem, List.mem_append, List.mem_bind] at hk
     obtain ⟨⟨k', v'⟩, ⟨(⟨a, ha₁, ha₂⟩|⟨a, ha₁, ha₂⟩), hk⟩⟩ := hk
     · obtain ⟨n, ⟨hn', hn⟩⟩ := List.getElem_of_mem ha₁
       rw [List.get_eq_get_append_right (self[i] :: l₂)] at hn
@@ -102,7 +101,7 @@ theorem exists_bucket_of_uset [BEq α] [Hashable α]
       rw [List.get_congr h₁.symm] at hn
       simp [← Array.getElem_eq_data_getElem] at hn
       refine (h.hashes_to (n + 1 + l₁.length) ?_).hash_self h₀ _ (hn.symm ▸ ha₂)
-      rw [Array.size_eq_length_data, h₁, length_append, length_cons]
+      rw [Array.size_eq_length_data, h₁, List.length_append, List.length_cons]
       omega
 
 theorem exists_bucket_of_update [BEq α] [Hashable α] (m : Array (AssocList α β)) (h : 0 < m.size) (k : α)
@@ -110,7 +109,7 @@ theorem exists_bucket_of_update [BEq α] [Hashable α] (m : Array (AssocList α 
     ∃ l : List (Σ a, β a),
       Perm (toListModel m) ((bucket m h k).toList ++ l) ∧
       Perm (toListModel (updateBucket m h k f)) ((f (bucket m h k)).toList ++ l) ∧
-      (∀ [LawfulHashable α], IsHashSelf m → ∀ k', hash k = hash k' → l.containsKey k' = false) := by
+      (∀ [LawfulHashable α], IsHashSelf m → ∀ k', hash k = hash k' → containsKey k' l = false) := by
   let idx := mkIdx m.size h (hash k)
   obtain ⟨l, h₁, h₂, h₃⟩ := exists_bucket_of_uset m idx.1 idx.2 (f m[idx.1])
   exact ⟨l, h₁, h₂, fun h k' hk' => h₃ h _ (hk' ▸ rfl)⟩
@@ -119,14 +118,14 @@ theorem exists_bucket' [BEq α] [Hashable α]
     (self : Array (AssocList α β)) (i : USize) (hi : i.toNat < self.size) :
       ∃ l, Perm (self.data.bind AssocList.toList) (self[i.toNat].toList ++ l) ∧
         (∀ [LawfulHashable α], IsHashSelf self → ∀ k,
-          (mkIdx self.size (by omega) (hash k)).1.toNat = i.toNat → l.containsKey k = false) := by
+          (mkIdx self.size (by omega) (hash k)).1.toNat = i.toNat → containsKey k l = false) := by
   obtain ⟨l, h₁, -, h₂⟩ := exists_bucket_of_uset self i hi .nil
   exact ⟨l, h₁, h₂⟩
 
 theorem exists_bucket [BEq α] [Hashable α]
     (m : Array (AssocList α β)) (h : 0 < m.size) (k : α) :
     ∃ l : List (Σ a, β a), Perm (toListModel m) ((bucket m h k).toList ++ l) ∧
-      (∀ [LawfulHashable α], IsHashSelf m → ∀ k', hash k = hash k' → l.containsKey k' = false) := by
+      (∀ [LawfulHashable α], IsHashSelf m → ∀ k', hash k = hash k' → containsKey k' l = false) := by
   obtain ⟨l, h₁, -, h₂⟩ := exists_bucket_of_update m h k (fun _ => .nil)
   exact ⟨l, h₁, h₂⟩
 
@@ -135,7 +134,7 @@ This is the general theorem used to show that access operations are correct.
 -/
 theorem apply_bucket [BEq α] [Hashable α] [PartialEquivBEq α] [LawfulHashable α] {m : Raw₀ α β} (hm : m.1.WFImp) {a : α}
     {f : AssocList α β → γ} {g : List (Σ a, β a) → γ} (hfg : ∀ {l}, f l = g l.toList)
-    (hg₁ : ∀ {l l'}, l.DistinctKeys → Perm l l' → g l = g l') (hg₂ : ∀ {l l'}, l'.containsKey a = false → g (l ++ l') = g l) :
+    (hg₁ : ∀ {l l'}, DistinctKeys l → Perm l l' → g l = g l') (hg₂ : ∀ {l l'}, containsKey a l' = false → g (l ++ l') = g l) :
     f (bucket m.1.buckets m.2 a) = g (toListModel m.1.buckets) := by
   obtain ⟨l, hl, hlk⟩ := exists_bucket m.1.buckets hm.buckets_size a
   refine Eq.trans ?_ (hg₁ (hm.distinct.perm hl.symm) hl.symm)
@@ -143,10 +142,10 @@ theorem apply_bucket [BEq α] [Hashable α] [PartialEquivBEq α] [LawfulHashable
   exact hlk hm.buckets_hash_self _ rfl
 
 theorem apply_bucket_with_proof {γ : α → Type w} [BEq α] [Hashable α] [PartialEquivBEq α] [LawfulHashable α] {m : Raw₀ α β} (hm : m.1.WFImp) (a : α)
-    (f : (a : α) → (l : AssocList α β) → l.contains a → γ a) (g : (a : α) → (l : List (Σ a, β a)) → l.containsKey a → γ a)
+    (f : (a : α) → (l : AssocList α β) → l.contains a → γ a) (g : (a : α) → (l : List (Σ a, β a)) → containsKey a l → γ a)
     (hfg : ∀ {a l h}, f a l h = g a l.toList (AssocList.contains_eq.symm.trans h))
-    (hg₁ : ∀ {l l' a h}, l.DistinctKeys → (hl' : Perm l l') → g a l h = g a l' ((List.containsKey_of_perm hl').symm.trans h)) {h h'}
-    (hg₂ : ∀ {l l' a h}, (hl' : l'.containsKey a = false) → g a (l ++ l') h = g a l ((List.containsKey_append_of_not_contains_right hl').symm.trans h)) :
+    (hg₁ : ∀ {l l' a h}, DistinctKeys l → (hl' : Perm l l') → g a l h = g a l' ((List.containsKey_of_perm hl').symm.trans h)) {h h'}
+    (hg₂ : ∀ {l l' a h}, (hl' : containsKey a l' = false) → g a (l ++ l') h = g a l ((List.containsKey_append_of_not_contains_right hl').symm.trans h)) :
     f a (bucket m.1.buckets m.2 a) h = g a (toListModel m.1.buckets) h' := by
   obtain ⟨l, hl, hlk⟩ := exists_bucket m.1.buckets hm.buckets_size a
   refine Eq.trans ?_ (hg₁ hm.distinct hl).symm
@@ -158,7 +157,7 @@ This is the general theorem to show that modification operations are correct.
 -/
 theorem toListModel_updateBucket [BEq α] [Hashable α] [PartialEquivBEq α] [LawfulHashable α] {m : Raw₀ α β} (hm : m.1.WFImp) {a : α}
     {f : AssocList α β → AssocList α β} {g : List (Σ a, β a) → List (Σ a, β a)} (hfg : ∀ {l}, (f l).toList = g l.toList)
-    (hg₁ : ∀ {l l'}, l.DistinctKeys → Perm l l' → Perm (g l) (g l')) (hg₂ : ∀ {l l'}, l'.containsKey a = false → g (l ++ l') = g l ++ l') :
+    (hg₁ : ∀ {l l'}, DistinctKeys l → Perm l l' → Perm (g l) (g l')) (hg₂ : ∀ {l l'}, containsKey a l' = false → g (l ++ l') = g l ++ l') :
     Perm (toListModel (updateBucket m.1.buckets m.2 a f)) (g (toListModel m.1.2)) := by
   obtain ⟨l, h₁, h₂, h₃⟩ := exists_bucket_of_update m.1.buckets m.2 a f
   refine h₂.trans (Perm.trans ?_ (hg₁ hm.distinct h₁).symm)
@@ -183,7 +182,7 @@ theorem toListModel_updateAllBuckets {m : Raw₀ α β} {f : AssocList α β →
   induction l generalizing l' l''
   · simpa using h.symm
   · next l t ih =>
-    simp only [foldl_cons]
+    simp only [List.foldl_cons]
     apply ih
     exact hg.trans (Perm.append h hfg.symm)
 
@@ -196,7 +195,7 @@ theorem mkArray [BEq α] [Hashable α] {c : Nat} : IsHashSelf (mkArray c (AssocL
   ⟨by simp⟩
 
 theorem uset [BEq α] [Hashable α] {m : Array (AssocList α β)} {i : USize} {h : i.toNat < m.size} {d : AssocList α β}
-    (hd : m[i].toList.HashesTo i.toNat m.size → d.toList.HashesTo i.toNat m.size) (hm : IsHashSelf m) : IsHashSelf (m.uset i d h) := by
+    (hd : HashesTo m[i].toList i.toNat m.size → HashesTo d.toList i.toNat m.size) (hm : IsHashSelf m) : IsHashSelf (m.uset i d h) := by
   refine ⟨fun j hj => ?_⟩
   simp only [Array.uset, Array.getElem_set, Array.size_set]
   split
@@ -207,8 +206,8 @@ theorem uset [BEq α] [Hashable α] {m : Array (AssocList α β)} {i : USize} {h
 This is the general theorem to show that modification operations preserve well-formedness of buckets.
 -/
 theorem updateBucket [BEq α] [Hashable α] [PartialEquivBEq α] [LawfulHashable α] {m : Array (AssocList α β)} {h : 0 < m.size} {a : α} {f : AssocList α β → AssocList α β}
-    (hf : ∀ l p, p ∈ (f l).toList → l.toList.containsKey p.1 ∨ hash p.1 = hash a) (hm : IsHashSelf m) : IsHashSelf (updateBucket m h a f) := by
-  rw [DHashMap.updateBucket]
+    (hf : ∀ l p, p ∈ (f l).toList → containsKey p.1 l.toList ∨ hash p.1 = hash a) (hm : IsHashSelf m) : IsHashSelf (updateBucket m h a f) := by
+  rw [Internal.updateBucket]
   refine IsHashSelf.uset (fun h' => ⟨fun _ p hp => ?_⟩) hm
   rcases hf _ _ hp with (hf|hf)
   · rw [containsKey_eq_true_iff_exists_mem] at hf
@@ -217,8 +216,8 @@ theorem updateBucket [BEq α] [Hashable α] [PartialEquivBEq α] [LawfulHashable
   · rw [hf]
 
 theorem updateAllBuckets [BEq α] [Hashable α] [LawfulHashable α] {m : Array (AssocList α β)} {f : AssocList α β → AssocList α δ}
-    (hf : ∀ l p, p ∈ (f l).toList → l.toList.containsKey p.1) (hm : IsHashSelf m) : IsHashSelf (updateAllBuckets m f) := by
-  rw [DHashMap.updateAllBuckets]
+    (hf : ∀ l p, p ∈ (f l).toList → containsKey p.1 l.toList) (hm : IsHashSelf m) : IsHashSelf (updateAllBuckets m f) := by
+  rw [Internal.updateAllBuckets]
   refine ⟨fun j hj => ?_⟩
   simp only [Array.getElem_map, Array.size_map]
   refine ⟨fun h p hp => ?_⟩
@@ -406,4 +405,4 @@ end
 
 end Raw₀
 
-end MyLean.DHashMap
+end MyLean.DHashMap.Internal
